02_FORMAL/coq/domains/SecureBootVerification.v
@@ -1,0 +1,111 @@
+(** ============================================================================
+    RIINA FORMAL VERIFICATION - SECURE BOOT VERIFICATION
+    File: SecureBootVerification.v | Theorems: 25 | Zero admits/axioms
+    ============================================================================ *)
+
+Require Import Coq.Bool.Bool.
+
+Lemma andb_true_iff : forall a b : bool, a && b = true <-> a = true /\ b = true.
+Proof. intros a b. split.
+  - intro H. destruct a; destruct b; simpl in *; split; try reflexivity; discriminate.
+  - intros [Ha Hb]. rewrite Ha, Hb. reflexivity.
+Qed.
+
+Record BootChain : Type := mkBootChain {
+  bc_rom_verified : bool; bc_bootloader_verified : bool;
+  bc_kernel_verified : bool; bc_initramfs_verified : bool;
+}.
+
+Record SecureBootConfig : Type := mkSecureBoot {
+  sb_chain : BootChain; sb_tpm_enabled : bool;
+  sb_measured_boot : bool; sb_remote_attestation : bool;
+}.
+
+Definition boot_chain_secure (b : BootChain) : bool :=
+  bc_rom_verified b && bc_bootloader_verified b && bc_kernel_verified b && bc_initramfs_verified b.
+
+Definition secure_boot_complete (s : SecureBootConfig) : bool :=
+  boot_chain_secure (sb_chain s) && sb_tpm_enabled s && sb_measured_boot s && sb_remote_attestation s.
+
+Definition riina_boot_chain : BootChain := mkBootChain true true true true.
+Definition riina_secure_boot : SecureBootConfig := mkSecureBoot riina_boot_chain true true true.
+
+Theorem SB_001 : boot_chain_secure riina_boot_chain = true. Proof. reflexivity. Qed.
+Theorem SB_002 : secure_boot_complete riina_secure_boot = true. Proof. reflexivity. Qed.
+Theorem SB_003 : bc_rom_verified riina_boot_chain = true. Proof. reflexivity. Qed.
+Theorem SB_004 : bc_bootloader_verified riina_boot_chain = true. Proof. reflexivity. Qed.
+Theorem SB_005 : bc_kernel_verified riina_boot_chain = true. Proof. reflexivity. Qed.
+Theorem SB_006 : bc_initramfs_verified riina_boot_chain = true. Proof. reflexivity. Qed.
+Theorem SB_007 : sb_tpm_enabled riina_secure_boot = true. Proof. reflexivity. Qed.
+Theorem SB_008 : sb_measured_boot riina_secure_boot = true. Proof. reflexivity. Qed.
+Theorem SB_009 : sb_remote_attestation riina_secure_boot = true. Proof. reflexivity. Qed.
+
+Theorem SB_010 : forall b, boot_chain_secure b = true -> bc_rom_verified b = true.
+Proof. intros b H. unfold boot_chain_secure in H. repeat (apply andb_true_iff in H; destruct H as [H _]). exact H. Qed.
+
+Theorem SB_011 : forall b, boot_chain_secure b = true -> bc_bootloader_verified b = true.
+Proof. intros b H. unfold boot_chain_secure in H.
+  apply andb_true_iff in H; destruct H as [H _].
+  apply andb_true_iff in H; destruct H as [H _].
+  apply andb_true_iff in H; destruct H as [_ H]. exact H. Qed.
+
+Theorem SB_012 : forall b, boot_chain_secure b = true -> bc_kernel_verified b = true.
+Proof. intros b H. unfold boot_chain_secure in H.
+  apply andb_true_iff in H; destruct H as [H _].
+  apply andb_true_iff in H; destruct H as [_ H]. exact H. Qed.
+
+Theorem SB_013 : forall b, boot_chain_secure b = true -> bc_initramfs_verified b = true.
+Proof. intros b H. unfold boot_chain_secure in H. apply andb_true_iff in H; destruct H as [_ H]. exact H. Qed.
+
+Theorem SB_014 : forall s, secure_boot_complete s = true -> boot_chain_secure (sb_chain s) = true.
+Proof. intros s H. unfold secure_boot_complete in H.
+  apply andb_true_iff in H; destruct H as [H _].
+  apply andb_true_iff in H; destruct H as [H _].
+  apply andb_true_iff in H; destruct H as [H _]. exact H. Qed.
+
+Theorem SB_015 : forall s, secure_boot_complete s = true -> sb_tpm_enabled s = true.
+Proof. intros s H. unfold secure_boot_complete in H.
+  apply andb_true_iff in H; destruct H as [H _].
+  apply andb_true_iff in H; destruct H as [H _].
+  apply andb_true_iff in H; destruct H as [_ H]. exact H. Qed.
+
+Theorem SB_016 : forall s, secure_boot_complete s = true -> sb_measured_boot s = true.
+Proof. intros s H. unfold secure_boot_complete in H.
+  apply andb_true_iff in H; destruct H as [H _].
+  apply andb_true_iff in H; destruct H as [_ H]. exact H. Qed.
+
+Theorem SB_017 : forall s, secure_boot_complete s = true -> sb_remote_attestation s = true.
+Proof. intros s H. unfold secure_boot_complete in H. apply andb_true_iff in H; destruct H as [_ H]. exact H. Qed.
+
+Theorem SB_018 : forall s, secure_boot_complete s = true -> bc_rom_verified (sb_chain s) = true.
+Proof. intros s H. apply SB_014 in H. apply SB_010 in H. exact H. Qed.
+
+Theorem SB_019 : forall s, secure_boot_complete s = true -> bc_kernel_verified (sb_chain s) = true.
+Proof. intros s H. apply SB_014 in H. apply SB_012 in H. exact H. Qed.
+
+Theorem SB_020 : forall b, boot_chain_secure b = true ->
+  bc_rom_verified b = true /\ bc_kernel_verified b = true.
+Proof. intros b H. split. apply SB_010. exact H. apply SB_012. exact H. Qed.
+
+Theorem SB_021 : forall s, secure_boot_complete s = true ->
+  sb_tpm_enabled s = true /\ sb_measured_boot s = true.
+Proof. intros s H. split. apply SB_015. exact H. apply SB_016. exact H. Qed.
+
+Theorem SB_022 : boot_chain_secure riina_boot_chain = true /\ sb_tpm_enabled riina_secure_boot = true.
+Proof. split; reflexivity. Qed.
+
+Theorem SB_023 : bc_rom_verified riina_boot_chain = true /\ bc_kernel_verified riina_boot_chain = true.
+Proof. split; reflexivity. Qed.
+
+Theorem SB_024 : sb_measured_boot riina_secure_boot = true /\ sb_remote_attestation riina_secure_boot = true.
+Proof. split; reflexivity. Qed.
+
+Theorem SB_025_complete : forall s, secure_boot_complete s = true ->
+  bc_rom_verified (sb_chain s) = true /\ bc_kernel_verified (sb_chain s) = true /\
+  sb_tpm_enabled s = true /\ sb_remote_attestation s = true.
+Proof. intros s H.
+  split. apply SB_018. exact H.
+  split. apply SB_019. exact H.
+  split. apply SB_015. exact H.
+  apply SB_017. exact H.
+Qed.
